deps/poulet4/lib/P4automata/Compiler.v
@@ -1,0 +1,208 @@
+Require Import Coq.Strings.String.
+Require Import Coq.Lists.List.
+
+Require Import Poulet4.P4cub.AST.
+Require Import Poulet4.P4cub.Value.
+Require Import Poulet4.Monads.Monad.
+Require Import Poulet4.Monads.Option.
+Require Import Poulet4.Monads.State.
+Require Import Poulet4.P4automata.P4automaton.
+
+Open Scope monad_scope.
+Open Scope string_scope.
+Open Scope list_scope.
+
+Section parser_to_p4automaton.
+
+  Variable tags_t : Type.
+
+  Inductive simple_expression :=
+  | SimpleExpressionHeader
+  | SimpleExpressionMember (e: simple_expression) (m: string)
+  .
+
+  Inductive simple_lvalue :=
+  | SimpleLvalueHeader
+  | SimpleLvalueMember (e: simple_lvalue) (m: string)
+  .
+
+  Inductive state_operation :=
+  | StateOperationNil
+  | StateOperationExtract
+      (typ: P4cub.Expr.t)
+      (into: simple_lvalue)
+  .
+
+  Inductive simple_match :=
+  | SimpleMatchEquals (l r: simple_expression)
+  | SimpleMatchAnd (l r: simple_match)
+  | SimpleMatchDontCare
+  .
+
+  Section compile.
+    Variables (pkt_name hdr_name: string).
+
+    Fixpoint compile_expression
+      (expr: P4cub.Expr.e tags_t)
+      : option simple_expression
+    :=
+      match expr with
+      | P4cub.Expr.EVar _ name _ =>
+        if name == hdr_name then
+          Some SimpleExpressionHeader
+        else
+          None
+      | P4cub.Expr.EExprMember name _ expr _ =>
+        let* child := compile_expression expr in
+        Some (SimpleExpressionMember child name)
+      | _ =>
+        None
+      end
+    .
+
+    Fixpoint compile_lvalue
+      (expr: P4cub.Expr.e tags_t)
+      : option simple_lvalue
+    :=
+      match expr with
+      | P4cub.Expr.EVar _ name _ =>
+        if name == hdr_name then
+          Some SimpleLvalueHeader
+        else
+          None
+      | P4cub.Expr.EExprMember name _ expr _ =>
+        let* child := compile_lvalue expr in
+        Some (SimpleLvalueMember child name)
+      | _ =>
+        None
+      end
+    .
+
+    Fixpoint compile_statements
+      (stmt: P4cub.Stmt.s tags_t)
+      : option (list state_operation)
+    :=
+      match stmt with
+      | P4cub.Stmt.SSkip _ =>
+        Some nil
+      | P4cub.Stmt.SSeq s1 s2 _ =>
+        let* f1 := compile_statements s1 in
+        let* f2 := compile_statements s2 in
+        Some (f1 ++ f2)
+      | P4cub.Stmt.SExternMethodCall extern func args _ =>
+        if extern == pkt_name then
+          if func == "extract" then
+            match args with
+            | P4cub.Arrow ((_, P4cub.PAOut (t, e)) :: nil) _ =>
+              let* into := compile_lvalue e in
+              Some (StateOperationExtract t into :: nil)
+            | _=> None
+            end
+          else
+            None
+        else
+          None
+      | _ => None
+      end
+    .
+
+    Fixpoint compile_updates
+      (states: Field.fs string (P4cub.Parser.ParserState.state_block tags_t))
+      : option (list (string * list state_operation))
+    :=
+      match states with
+      | nil =>
+        Some nil
+      | state :: states' =>
+        let '(name, P4cub.Parser.ParserState.State stmt _) := state in
+        let* tail := compile_updates states' in
+        let* head := compile_statements stmt in
+        Some ((name, head) :: tail)
+      end
+    .
+
+    Section NotationSection.
+    Import P4cub.P4cubNotations.
+
+    Fixpoint compile_transition
+      (trans: P4cub.Parser.ParserState.e tags_t)
+      : option (list (simple_match * (string + bool)))
+    :=
+      match trans with
+      | p{ goto start @ _ }p => None (* TODO: Implement this. *)
+      | p{ goto accept @ _ }p =>
+        Some ((SimpleMatchDontCare, inr true) :: nil)
+      | p{ goto reject @ _ }p =>
+        Some ((SimpleMatchDontCare, inr false) :: nil)
+      | p{ goto δ st @ _ }p =>
+        Some ((SimpleMatchDontCare, inl st) :: nil)
+      | p{ select select_exp { cases } default:=def @ _ }p =>
+        let* select_exp' := compile_expression select_exp in
+        let fix f cases :=
+          match cases with
+          | nil =>
+            compile_transition def
+          | (case_exp, case_trans) :: cases' =>
+            let* child_clauses := compile_transition case_trans in
+            let* case_exp' := compile_expression case_exp in
+            let augmented_clauses :=
+              map (
+                fun '(clause, target) =>
+                (SimpleMatchAnd (SimpleMatchEquals select_exp' case_exp')
+                                clause,
+                 target)
+              ) child_clauses in
+            let* tail := f cases' in
+            Some (augmented_clauses ++ tail)
+          end in
+         f cases
+      end
+    .
+    End NotationSection.
+
+    Fixpoint compile_transitions
+      (states: Field.fs string (P4cub.Parser.ParserState.state_block tags_t))
+      : option (list (string * list (simple_match * (string + bool))))
+    :=
+      match states with
+      | nil =>
+        Some nil
+      | state :: states' =>
+        let '(name, P4cub.Parser.ParserState.State _ trans) := state in
+        let* tail := compile_transitions states' in
+        let* head := compile_transition trans in
+        Some ((name, head) :: tail)
+      end
+    .
+
+  End compile.
+
+  Record embedded_p4automaton := MkEmbeddedP4Automaton {
+    emb_updates: list (string * list state_operation);
+    emb_transitions: list (string * list (simple_match * (string + bool)));
+  }.
+
+  Definition parser_to_p4automaton
+    (parser: P4cub.TopDecl.d tags_t)
+    : option embedded_p4automaton
+  :=
+    match parser with
+    | P4cub.TopDecl.TPParser _ _ params _ states _ => (* AST.v change *)
+      match params with
+      | (pkt_name, P4cub.PAIn pkt_type) ::
+        (hdr_name, P4cub.PAOut hdr_type) :: _ =>
+        let* updates := compile_updates pkt_name hdr_name states in
+        let* transitions := compile_transitions hdr_name states in
+        Some {|
+          emb_updates := updates;
+          emb_transitions := transitions;
+        |}
+      | _ =>
+        None
+      end
+    | _ =>
+      None
+    end
+  .
+
+End parser_to_p4automaton.
