deps/poulet4/lib/P4automata/P4automaton.v
@@ -1,0 +1,179 @@
+Require Import Coq.Lists.List.
+Require Import Coq.Classes.EquivDec.
+
+Record p4automaton := MkP4Automaton {
+  store: Type;
+  states: Type;
+  size: states -> nat;
+  update: states -> list bool -> store -> store;
+  transitions: states -> store -> states + bool;
+}.
+
+Definition configuration (a: p4automaton) : Type :=
+  (states a + bool) * store a * list bool
+.
+
+Definition step
+  {a: p4automaton}
+  (c: configuration a)
+  (b: bool)
+  : configuration a
+:=
+  let '(state, st, buf) := c in
+  match state with
+  | inl state =>
+    let buf' := buf ++ b :: nil in
+    if List.length buf' == size a state
+    then
+      let st' := update a state buf' st in
+      let state' := transitions a state st' in
+      (state', st', nil)
+    else (inl state, st, buf')
+  | inr halt =>
+    (inr halt, st, buf ++ b :: nil)
+  end
+.
+
+Definition follow
+  {a: p4automaton}
+  (c: configuration a)
+  (input: list bool)
+  : configuration a
+:=
+  fold_left step input c
+.
+
+Lemma follow_cons
+  {a: p4automaton}
+  (c: configuration a)
+  (b: bool)
+  (input: list bool)
+:
+  follow c (b :: input) = follow (step c b) input
+.
+Proof.
+  reflexivity.
+Qed.
+
+Definition accepting
+  {a: p4automaton}
+  (c: configuration a)
+  : Prop
+:=
+  fst (fst c) = inr true
+.
+
+Definition accepted
+  {a: p4automaton}
+  (c: configuration a)
+  (input: list bool)
+  : Prop
+:=
+  accepting (follow c input)
+.
+
+Definition lang_equiv
+  {a1: p4automaton}
+  {a2: p4automaton}
+  (c1: configuration a1)
+  (c2: configuration a2)
+:=
+  forall input,
+    accepted c1 input <->
+    accepted c2 input
+.
+
+Definition bisimulation
+  {a1: p4automaton}
+  {a2: p4automaton}
+  (R: configuration a1 -> configuration a2 -> Prop)
+:=
+  forall c1 c2,
+    R c1 c2 ->
+      (accepting c1 <-> accepting c2) /\
+      forall b, R (step c1 b) (step c2 b)
+.
+
+Definition bisimilar
+  {a1: p4automaton}
+  {a2: p4automaton}
+  (c1: configuration a1)
+  (c2: configuration a2)
+:=
+  exists R, bisimulation R /\ R c1 c2
+.
+
+Lemma bisimilar_implies_equiv
+  {a1: p4automaton}
+  {a2: p4automaton}
+  (c1: configuration a1)
+  (c2: configuration a2)
+:
+  bisimilar c1 c2 -> lang_equiv c1 c2
+.
+Proof.
+  intros.
+  unfold lang_equiv.
+  intros; revert c1 c2 H.
+  induction input; intros.
+  - unfold accepted.
+    simpl.
+    unfold bisimilar in H.
+    destruct H as [R [? ?]].
+    now apply H in H0.
+  - unfold accepted.
+    repeat rewrite follow_cons.
+    apply IHinput.
+    unfold bisimilar in H.
+    destruct H as [R [? ?]].
+    exists R.
+    apply H in H0.
+    easy.
+Qed.
+
+Lemma lang_equiv_is_bisimulation
+  {a1: p4automaton}
+  {a2: p4automaton}
+:
+  @bisimulation a1 a2 lang_equiv
+.
+Proof.
+  unfold bisimulation; intros.
+  split.
+  - apply (H nil).
+  - intros.
+    unfold lang_equiv.
+    intros.
+    unfold accepted.
+    repeat rewrite <- follow_cons.
+    apply H.
+Qed.
+
+Lemma equiv_implies_bisimilar
+  {a1: p4automaton}
+  {a2: p4automaton}
+  (c1: configuration a1)
+  (c2: configuration a2)
+:
+  lang_equiv c1 c2 -> bisimilar c1 c2
+.
+Proof.
+  intros.
+  exists lang_equiv.
+  split; try easy.
+  apply lang_equiv_is_bisimulation.
+Qed.
+
+Theorem bisimilar_iff_lang_equiv
+  {a1: p4automaton}
+  {a2: p4automaton}
+  (c1: configuration a1)
+  (c2: configuration a2)
+:
+  lang_equiv c1 c2 <-> bisimilar c1 c2
+.
+Proof.
+  split.
+  - apply equiv_implies_bisimilar.
+  - apply bisimilar_implies_equiv.
+Qed.
